Project.v
@@ -100,12 +100,11 @@ Hint Constructors value_or_abs.
 (** To prove that the machine terminates, we assume that weak reduction terminates,
     and then show that the machine simulates weak reduction (in bigstep semantics) *)
 
-Axiom weak_terminates :
-  forall M, well_typed M ->
+Axiom weak_terminates : forall M,
+  well_typed M ->
   exists W, M -w->* W /\ value_or_abs W.
 
-Lemma app_cons_app {A} :
-  forall (l1 l2 : list A) (a : A),
+Lemma app_cons_app {A} : forall (l1 l2 : list A) (a : A),
   l1 ++ a :: l2 = (l1 ++ [a]) ++ l2.
 Proof.
   induction l1, l2; firstorder.
@@ -113,8 +112,7 @@ Proof.
   rewrite app_comm_cons. reflexivity.
 Qed.
 
-Remark step_stack_closure π :
-  forall M1 π1 M2 π2,
+Remark step_stack_closure π : forall M1 π1 M2 π2,
   (M1 ⊣ π1 -k->* M2 ⊣ π2) -> (M1 ⊣ π1 ++ π -k->* M2 ⊣ π2 ++ π).
 Proof.
   induction π.
@@ -138,9 +136,9 @@ Fixpoint stack_of_context E :=
   | CIf E N z P => stack_of_context E ++ [If N z P]
   end.
 
-Lemma step_simulates_weak_comp E :
+Lemma step_simulates_weak_comp E : forall M N,
   let π := stack_of_context E in
-  forall M N, M --> N -> E[M] ⊣ [] -k->* N ⊣ π.
+  M --> N -> E[M] ⊣ [] -k->* N ⊣ π.
 Proof.
   intros. induction E; simpl in *.
   * destruct H; econstructor; eauto.
@@ -156,9 +154,9 @@ Proof.
     rewrite <- app_nil_l with (l := [If N0 z P]). apply step_stack_closure. assumption.
 Qed.
 
-Lemma step_context_to_stack E :
+Lemma step_context_to_stack E : forall M,
   let π := stack_of_context E in
-  forall M, E[M] ⊣ [] -k->* M ⊣ π.
+  E[M] ⊣ [] -k->* M ⊣ π.
 Proof.
   intros. induction E; simpl in *.
   * apply multistep_refl.
@@ -177,9 +175,8 @@ Qed.
 Definition normal_form_step M π :=
   ~ exists M' π', M ⊣ π -k-> M' ⊣ π'.
 
-Lemma value_or_abs_normal_form_step :
-  forall W, value_or_abs W ->
-  normal_form_step W ([]).
+Lemma value_or_abs_normal_form_step W :
+  value_or_abs W -> normal_form_step W ([]).
 Proof.
   intros. intro. destruct H0 as (M' & π' & H0). destruct H.
   * destruct H; inversion H0.
@@ -190,8 +187,7 @@ Lemma multistep_deterministic : TODO _.
 Proof.
 Admitted.
 
-Lemma one_way_to_normal_form :
-  forall M1 π1 M2 π2 M3 π3,
+Lemma one_way_to_normal_form : forall M1 π1 M2 π2 M3 π3,
   (M1 ⊣ π1 -k->* M3 ⊣ π3) -> (normal_form_step M3 π3) ->
   (M1 ⊣ π1 -k->* M2 ⊣ π2) ->
   (M2 ⊣ π2 -k->* M3 ⊣ π3).
@@ -199,8 +195,8 @@ Proof.
   (* The proof will use multistep_deterministic *)
 Admitted.
 
-Theorem step_simulates_weak_bigstep :
-  forall M W, value_or_abs W ->
+Theorem step_simulates_weak_bigstep : forall M W,
+  value_or_abs W ->
   M -w->* W -> M ⊣ [] -k->* W ⊣ [].
 Proof.
   intros. induction H0 as [ M | M N W ].
@@ -213,8 +209,8 @@ Proof.
     apply multistep_trans with (M2 := N) (π2 := stack_of_context E); assumption.
 Qed.
 
-Theorem step_terminates :
-  forall M, well_typed M ->
+Theorem step_terminates : forall M,
+  well_typed M ->
   exists N, (M ⊣ [] -k->* N ⊣ []) /\ normal_form_step N ([]).
 Proof.
   intros.
@@ -235,7 +231,7 @@ Bind Scope eval_scope with state.
 
 Notation "M -| π" := (State M π Running) (at level 80) : machine_scope.
 
-Definition fstep (s : state) : state :=
+Definition eval_step (s : state) : state :=
   match s with
   (* Stack update rules *)
   | (der M -| π) => M -| Der :: π
@@ -255,13 +251,33 @@ Definition fstep (s : state) : state :=
   | State M π _ => State M π Done
   end.
 
+Lemma eval_step_simulates_step : forall M π M' π',
+  (M ⊣ π -k-> M' ⊣ π') ->
+  eval_step (M -| π) = (M' -| π').
+Proof.
+  destruct 1; simpl; auto.
+  * destruct H; auto. destruct n; auto.
+  * destruct n; auto.
+Qed.
+
 Fixpoint run (fuel : nat) (s : state) { struct fuel } : state :=
-  let s := fstep s in
   let (M, π, status) := s in
   match fuel, status with
-  | S n, Running => run n (M -| π)
-  | _, _ => s
+  | 0, _ | S _, Done => State M π Done
+  | S n, Running => run n (eval_step s)
   end.
+
+Lemma run_simulates_step : forall M π V,
+  value V ->
+  (M ⊣ π -k->* V ⊣ []) ->
+  exists n, run n (M -| π) = State V ([]) Done.
+Proof.
+  induction 2.
+  * exists 0. simpl. reflexivity.
+  * apply eval_step_simulates_step in H0. apply IHmultistep in H.
+    destruct H as (n & ?). exists (S n).
+    unfold run. rewrite H0. fold run. assumption.
+Qed.
 
 Fixpoint unstack M π :=
   match π with
@@ -284,31 +300,90 @@ Definition eval (fuel : nat) (s : state) : term :=
   | _ => let (V', _, _) := unstack V π in V'
   end.
 
-Theorem eval_invariant_by_step :
-  forall M π M' π', (M ⊣ π -k-> M' ⊣ π') ->
-  exists n, eval n (M -| π) = eval n (M' -| π').
-Proof.
-  intros.
-Admitted.
-
-Theorem eval_simulates_step :
-  forall M π V, value V -> (M ⊣ π -k->* V ⊣ []) ->
+Lemma eval_simulates_one_step : forall M π V,
+  value V ->
+  (M ⊣ π -k-> V ⊣ []) ->
   exists n, eval n (M -| π) = V.
 Proof.
-  intros.
+  intros. eapply multistep_step in H0; eauto.
+  pose proof (run_simulates_step M π V H H0).
+  destruct H1 as (n & ?). exists n. unfold eval.
+  destruct (run n (M -| π)). inversion_clear H1. auto.
+Qed.
+
+Theorem eval_simulates_step : forall M π V,
+  value V ->
+  (M ⊣ π -k->* V ⊣ []) ->
+  exists n, eval n (M -| π) = V.
+Proof.
+  intros. pose proof (run_simulates_step M π V H H0).
+  destruct H1 as (n & ?). exists n. unfold eval.
+  destruct (run n (M -| π)). inversion_clear H1. auto.
+Qed.
+
+Lemma eval_terminates : forall M π,
+  exists n M', eval n (M -| π) = M'.
+Proof.
 Admitted.
+
+Lemma run_eval_step : forall M π M' π',
+  eval_step (M -| π) = (M' -| π') ->
+  exists n, run n (M -| π) = run n (eval_step (M -| π)).
+Proof.
+  intros. destruct (eval_terminates M π) as (n & P & ?).
+  exists n. unfold run at 1.
+Admitted.
+
+Lemma run_invariant_by_step : forall M π M' π',
+  (M ⊣ π -k-> M' ⊣ π') ->
+  exists n, run n (M -| π) = run n (M' -| π').
+Proof.
+  intros.
+  pose proof (eval_step_simulates_step M π M' π' H).
+  destruct (run_eval_step M π M' π' H0) as (n & ?).
+  exists n. rewrite H1. rewrite H0. reflexivity.
+Qed.
+
+Theorem eval_invariant_by_step : forall M π M' π',
+  (M ⊣ π -k-> M' ⊣ π') ->
+  exists n, eval n (M -| π) = eval n (M' -| π').
+Proof.
+  intros. destruct (run_invariant_by_step M π M' π' H) as (n & ?).
+  exists n. unfold eval. rewrite H0. reflexivity.
+Qed.
 
 (** Question 4 *)
 
 Inductive valid_stack_judgment : general -> stack -> general -> Prop :=
 
-| Todo σ π τ : σ ⊢ π : τ
+| T_Empty τ :
+  τ ⊢ [] : τ
+
+| T_Der σ π τ :
+  σ ⊢ π : τ ->
+  !σ ⊢ (Der :: π) : τ
+
+| T_Succ π τ :
+  ι ⊢ π : τ ->
+  ι ⊢ (Succ :: π) : τ
+
+| T_Arg (φ : positive) σ V π τ :
+  ([] ⊢ V : φ)%typing -> σ ⊢ π : τ ->
+  (φ -o σ) ⊢ (Arg V :: π) : τ
+
+| T_Fun (φ : positive) M π τ σ :
+  ([] ⊢ M : φ -o σ)%typing -> σ ⊢ π : τ ->
+  φ ⊢ (Fun M :: π) : τ
+
+| T_If N z P π τ σ :
+  ([] ⊢ N : σ)%typing -> ([z : ι] ⊢ P : σ)%typing -> σ ⊢ π : τ ->
+  ι ⊢ (If N z P :: π) : τ
 
 where "σ ⊢ π : τ" := (valid_stack_judgment σ π τ) : machine_scope.
 
 Hint Constructors valid_stack_judgment.
 
-Reserved Notation "⊢ ( M , π ) : σ" (at level 100, π at level 90, σ at level 90).
+Reserved Notation "⊢ ( M , π )  : σ" (at level 100, π at level 90, σ at level 90).
 
 Inductive valid_state_judgment : term -> stack -> general -> Prop :=
 
@@ -318,17 +393,138 @@ Inductive valid_state_judgment : term -> stack -> general -> Prop :=
 
 where "⊢ ( M , π ) : σ" := (valid_state_judgment M π σ) : machine_scope.
 
-Theorem step_subject_reduction σ :
-  forall M π M' π',
+Open Scope typing_scope.
+
+Definition subcontext (Γ Γ' : Typing.context) :=
+  forall a, List.In a Γ -> List.In a Γ'.
+
+Notation "Γ ⊂ Γ'" := (subcontext Γ Γ') (at level 60) : typing_scope.
+
+Lemma valid_judgment_Wf_context Γ : forall M σ,
+  Γ ⊢ M : σ -> Wf_context Γ.
+Proof.
+  induction 1; auto. firstorder.
+Qed.
+
+Lemma Wf_context_subcontext Γ Γ' :
+  Γ' ⊂ Γ ->
+  Wf_context Γ -> Wf_context Γ'.
+Proof.
+  unfold Wf_context. intros. apply (H0 a a') in H; auto.
+Qed.
+
+Lemma exchange x φ y ψ : forall Γ M σ,
+  (x : φ :: y : ψ :: Γ) ⊢ M : σ <->
+  (y : ψ :: x : φ :: Γ) ⊢ M : σ.
+Proof.
+  intros. split.
+  * induction 1; auto.
+Admitted.
+
+Lemma weakening Γ Γ' :
+  Γ ⊂ Γ' -> Wf_context Γ' ->
+  forall M σ, Γ ⊢ M : σ -> Γ' ⊢ M : σ.
+Proof.
+  induction 3; auto.
+  * destruct σ; intuition.
+  * econstructor.
+Admitted.
+
+Lemma subst_typing :
+  forall M σ V (φ : positive) x Γ (HWf : Wf_context Γ),
+  (x : φ :: Γ) ⊢ M : σ -> Γ ⊢ V : φ ->
+  Γ ⊢ M[V/x] : σ.
+Proof.
+  induction M; intros; simpl; inversion H; try (econstructor; eauto).
+  * destruct σ.
+    - case (x0 =? x) eqn:?.
+      + apply eqb_eq in Heqb. destruct H4.
+        ** congruence.
+        ** admit. (* The proof would be by case on φ =? φ0,
+                     but we don't have the decidable equality
+                     on types yet... *)
+      + apply eqb_neq in Heqb. destruct H4.
+        ** congruence.
+        ** constructor; assumption.
+    - contradiction.
+  * case (x0 =? x) eqn:?.
+    - apply eqb_eq in Heqb. admit.
+      (* Again a proof by case on φ =? φ0 *)
+    - assert (Wf_context (x : φ :: Γ)).
+      { apply valid_judgment_Wf_context in H6.
+        eapply Wf_context_subcontext; eauto.
+        unfold "⊂". intros. destruct H7.
+        left. assumption. right. right. assumption. }
+      apply eqb_neq in Heqb. eapply IHM; eauto.
+      + apply exchange. eauto.
+      + eapply weakening; eauto.
+        unfold "⊂". intros. right. assumption.
+  * case (x =? z) eqn:?.
+    - apply eqb_eq in Heqb. admit.
+      (* Again a proof by case on φ =? ι *)
+    - assert (Wf_context (z : ι :: Γ)).
+      { apply valid_judgment_Wf_context in H9.
+        eapply Wf_context_subcontext; eauto.
+        unfold "⊂". intros. destruct H10.
+        left. assumption. right. right. assumption. }
+      apply eqb_neq in Heqb. eapply IHM3; eauto.
+      + apply exchange. eauto.
+      + eapply weakening; eauto.
+        unfold "⊂". intros. right. assumption.
+Admitted.
+
+Close Scope typing_scope.
+
+Theorem step_subject_reduction σ : forall M π M' π',
   ⊢ (M, π) : σ -> (M ⊣ π -k-> M' ⊣ π') ->
   ⊢ (M', π') : σ.
 Proof.
-Admitted.
+  destruct 2; inversion H.
+  * inversion H0. econstructor; eauto.
+  * inversion H0. econstructor; eauto. econstructor. congruence.
+  * inversion H0. econstructor; eauto.
+  * inversion H2. econstructor; eauto. econstructor; eauto. congruence.
+  * inversion H0. econstructor; eauto.
+  * inversion H0. inversion H1. econstructor; eauto. congruence.
+  * inversion H0. inversion H1. econstructor; eauto.
+  * inversion H1. inversion H2. econstructor; eauto.
+    eapply subst_typing; eauto; try easy. congruence.
+  * inversion H0. inversion H1. econstructor; eauto.
+  * inversion H0. inversion H1. econstructor; eauto.
+    eapply subst_typing; eauto.
+Qed.
 
-Theorem eval_subject_reduction σ :
-  forall M π, ⊢ (M, π) : σ ->
+Theorem eval_subject_reduction σ : forall M π,
+  ⊢ (M, π) : σ ->
   exists n, ([] ⊢ eval n (M -| π) : σ)%typing.
 Proof.
+  destruct 1.
 Admitted.
 
+End ΛHP_Machine.
+
 (** Question 6 *)
+
+Module Λv.
+
+Module Types.
+
+Inductive type :=
+| TNat
+| TArrow (A : type) (B : type).
+
+Hint Constructors type.
+
+End Types.
+
+Module Terms.
+
+End Terms.
+
+End Λv.
+
+(** Question 7 *)
+
+Module Λn.
+
+End Λn.
